\documentclass{article}
\begin{document}

\title{Solution to Shreenabh Agrawal's Daily Challenge 6}
\author{Jose Bedoya}
\maketitle

\vspace{10mm}

{\small

$$\int_{0}^{1} \ln{x}\ln{(1-x)}\,dx$$
\vspace{5mm}
Knowing,
$$\sum_{k=1}^{\infty} x^{k-1} = \frac{1}{1-x}\,, \hspace{2mm} |x|<1$$
Integrating both sides:
$$\sum_{k=1}^{\infty} \frac{x^k}{k} = -\ln{(1-x)}$$
Therefore,
$$\int_{0}^{1} \ln{x}\ln{(1-x)}\,dx = \int_{0}^{1} \ln{x}\,\left(-\sum_{k=1}^{\infty} \frac{x^k}{k}\right)\,dx$$
Here we can change the order of integration and summation (think of it in an intuitive way)
$$= -\sum_{k=1}^{\infty}\frac{1}{k}\int_{0}^{1} x^k\ln{x}\,dx$$
Applying IBP,
$$=-\sum_{k=1}^{\infty} \frac{1}{k}\left(\frac{x^{k+1}\ln x}{k+1}\Big|_0^1 -\frac{1}{k+1}\int_{0}^{1}x^{k} \,dx \right)$$
$$=\sum_{k=1}^{\infty} \frac{1}{k(k+1)^2}$$
$$=\sum_{k=1}^{\infty} \frac{k+1-k}{k(k+1)^2}=\sum_{k=1}^{\infty}\frac{1}{k(k+1)} - \sum_{k=1}^{\infty}\frac{1}{(k+1)^2}$$

\vspace{2mm}
The first sum is telescopic, this means
$$\sum_{k=1}^{\infty}\frac{1}{k(k+1)}=\sum_{k=1}^{\infty} \left(\frac{1}{k}-\frac{1}{k+1}\right)= \lim_{n\to\infty}\left(1-\frac{1}{2}+\frac{1}{2}-\frac{1}{3}+\cdots + \frac{1}{n}-\frac{1}{n+1}\right)$$
$$\sum_{k=1}^{\infty}\frac{1}{k(k+1)}=1$$
As for the second sum, we know the Riemann Zeta Function evaluated at $s$ is 

$$\zeta(s)=\sum_{k=1}^{\infty} \frac{1}{k^s}$$

Therefore,
$$\sum_{k=1}^{\infty} \frac{1}{(k+1)^2}=\zeta(2)-1$$
And,
$$\zeta(2)=\frac{\pi^2}{6}$$
Thus, our final answer is

$$\int_{0}^{1} \ln x \ln{(1-x})\,dx = 2-\frac{\pi^2}{6}$$
}
\end{document}